PSLC

src/Interps.v
@@ -61,7 +61,7 @@ Module STLC.
   Notation "# v" := (Var v) (at level 70).
 
   Notation "^ n" := (Const n) (at level 70).
-  Infix "++" := Plus.
+  Infix "+^" := Plus (left associativity, at level 79).
 
   Infix "@" := App (left associativity, at level 77).
   Notation "\ x , e" := (Abs (fun x => e)) (at level 78).
@@ -99,7 +99,7 @@ Module STLC.
           let e2' := cfold e2 in
           match e1', e2' with
             | Const n1, Const n2 => ^(n1 + n2)
-            | _, _ => e1' ++ e2'
+            | _, _ => e1' +^ e2'
           end
 
         | App _ _ e1 e2 => cfold e1 @ cfold e2
@@ -122,3 +122,166 @@ Module STLC.
     unfold ExpDenote, Cfold; intros; apply cfold_correct.
   Qed.
 End STLC.
+
+
+(** * Adding Products and Sums *)
+
+Module PSLC.
+  Inductive type : Type :=
+  | Nat : type
+  | Arrow : type -> type -> type
+  | Prod : type -> type -> type
+  | Sum : type -> type -> type.
+
+  Infix "-->" := Arrow (right associativity, at level 62).
+  Infix "**" := Prod (right associativity, at level 61).
+  Infix "++" := Sum (right associativity, at level 60).
+
+  Section vars.
+    Variable var : type -> Type.
+
+    Inductive exp : type -> Type :=
+    | Var : forall t,
+      var t
+      -> exp t
+
+    | Const : nat -> exp Nat
+    | Plus : exp Nat -> exp Nat -> exp Nat
+
+    | App : forall t1 t2,
+      exp (t1 --> t2)
+      -> exp t1
+      -> exp t2
+    | Abs : forall t1 t2,
+      (var t1 -> exp t2)
+      -> exp (t1 --> t2)
+
+    | Pair : forall t1 t2,
+      exp t1
+      -> exp t2
+      -> exp (t1 ** t2)
+    | Fst : forall t1 t2,
+      exp (t1 ** t2)
+      -> exp t1
+    | Snd : forall t1 t2,
+      exp (t1 ** t2)
+      -> exp t2
+
+    | Inl : forall t1 t2,
+      exp t1
+      -> exp (t1 ++ t2)
+    | Inr : forall t1 t2,
+      exp t2
+      -> exp (t1 ++ t2)
+    | SumCase : forall t1 t2 t,
+      exp (t1 ++ t2)
+      -> (var t1 -> exp t)
+      -> (var t2 -> exp t)
+      -> exp t.
+  End vars.
+
+  Definition Exp t := forall var, exp var t.
+
+  Implicit Arguments Var [var t].
+  Implicit Arguments Const [var].
+  Implicit Arguments Abs [var t1 t2].
+  Implicit Arguments Inl [var t1 t2].
+  Implicit Arguments Inr [var t1 t2].
+
+  Notation "# v" := (Var v) (at level 70).
+
+  Notation "^ n" := (Const n) (at level 70).
+  Infix "+^" := Plus (left associativity, at level 79).
+
+  Infix "@" := App (left associativity, at level 77).
+  Notation "\ x , e" := (Abs (fun x => e)) (at level 78).
+  Notation "\ ! , e" := (Abs (fun _ => e)) (at level 78).
+
+  Notation "[ e1 , e2 ]" := (Pair e1 e2).
+  Notation "#1 e" := (Fst e) (at level 75).
+  Notation "#2 e" := (Snd e) (at level 75).
+
+  Notation "'case' e 'of' x => e1 | y => e2" := (SumCase e (fun x => e1) (fun y => e2))
+    (at level 79).
+
+  Fixpoint typeDenote (t : type) : Set :=
+    match t with
+      | Nat => nat
+      | t1 --> t2 => typeDenote t1 -> typeDenote t2
+      | t1 ** t2 => typeDenote t1 * typeDenote t2
+      | t1 ++ t2 => typeDenote t1 + typeDenote t2
+    end%type.
+
+  Fixpoint expDenote t (e : exp typeDenote t) {struct e} : typeDenote t :=
+    match e in (exp _ t) return (typeDenote t) with
+      | Var _ v => v
+        
+      | Const n => n
+      | Plus e1 e2 => expDenote e1 + expDenote e2
+        
+      | App _ _ e1 e2 => (expDenote e1) (expDenote e2)
+      | Abs _ _ e' => fun x => expDenote (e' x)
+
+      | Pair _ _ e1 e2 => (expDenote e1, expDenote e2)
+      | Fst _ _ e' => fst (expDenote e')
+      | Snd _ _ e' => snd (expDenote e')
+
+      | Inl _ _ e' => inl _ (expDenote e')
+      | Inr _ _ e' => inr _ (expDenote e')
+      | SumCase _ _ _ e' e1 e2 =>
+        match expDenote e' with
+          | inl v => expDenote (e1 v)
+          | inr v => expDenote (e2 v)
+        end
+    end.
+
+  Definition ExpDenote t (e : Exp t) := expDenote (e _).
+
+  Section cfold.
+    Variable var : type -> Type.
+
+    Fixpoint cfold t (e : exp var t) {struct e} : exp var t :=
+      match e in exp _ t return exp _ t with
+        | Var _ v => #v
+
+        | Const n => ^n
+        | Plus e1 e2 =>
+          let e1' := cfold e1 in
+          let e2' := cfold e2 in
+          match e1', e2' with
+            | Const n1, Const n2 => ^(n1 + n2)
+            | _, _ => e1' +^ e2'
+          end
+
+        | App _ _ e1 e2 => cfold e1 @ cfold e2
+        | Abs _ _ e' => Abs (fun x => cfold (e' x))
+
+        | Pair _ _ e1 e2 => [cfold e1, cfold e2]
+        | Fst _ _ e' => #1 (cfold e')
+        | Snd _ _ e' => #2 (cfold e')
+
+        | Inl _ _ e' => Inl (cfold e')
+        | Inr _ _ e' => Inr (cfold e')
+        | SumCase _ _ _ e' e1 e2 =>
+          case cfold e' of
+            x => cfold (e1 x)
+          | y => cfold (e2 y)
+      end.
+  End cfold.
+
+  Definition Cfold t (E : Exp t) : Exp t := fun _ => cfold (E _).
+
+  Lemma cfold_correct : forall t (e : exp _ t),
+    expDenote (cfold e) = expDenote e.
+    induction e; crush; try (ext_eq; crush);
+      repeat (match goal with
+                | [ |- context[cfold ?E] ] => dep_destruct (cfold E)
+                | [ |- match ?E with inl _ => _ | inr _ => _ end = _ ] => destruct E
+              end; crush).
+  Qed.
+
+  Theorem Cfold_correct : forall t (E : Exp t),
+    ExpDenote (Cfold E) = ExpDenote E.
+    unfold ExpDenote, Cfold; intros; apply cfold_correct.
+  Qed.
+End PSLC.
